theories/LogicalRelation/Irrelevance.v
@@ -180,6 +180,9 @@ Proof.
   intros []; cbn in *; unshelve econstructor; tea.
   - intros; unshelve eapply eqv.(eqvShp); now auto.
   - now eapply redtmwf_conv.
+  - destruct isfun as [A₀ t₀|n Hn].
+    + constructor; transitivity (PiRedTy.dom ΣA); [now symmetry|tea].
+    + now constructor.
   - now eapply convtm_conv.
   - intros; unshelve eapply eqv.(eqvPos); now auto.
 Defined.
